wip

code/ecdsap256sha2/Hacl.Impl.LowLevel.fst
@@ -126,6 +126,8 @@ let load_buffer8 a0 a1 a2 a3 a4 a5 a6 a7  o =
   upd o (size 7) a7
 
 (** This is unused *)
+(** Now it's used*)
+
 inline_for_extraction noextract
 val copy_conditional_u64: a: uint64 -> b: uint64 -> mask: uint64 {uint_v mask = 0 \/ uint_v mask = pow2 64 - 1} -> 
   Tot (r: uint64 {if uint_v mask = 0 then uint_v r = uint_v a else uint_v r = uint_v b})
@@ -133,6 +135,7 @@ val copy_conditional_u64: a: uint64 -> b: uint64 -> mask: uint64 {uint_v mask = 
 let copy_conditional_u64 a b mask = 
   lemma_xor_copy_cond a b mask;
   logxor a (logand mask (logxor a b))
+
 
 val copy_conditional: out: felem -> x: felem -> mask: uint64{uint_v mask = 0 \/ uint_v mask = pow2 64 - 1} -> Stack unit 
   (requires fun h -> live h out /\ live h x)
@@ -171,7 +174,7 @@ let copy_conditional out x mask =
   lemma_eq_funct_ (as_seq h1 out) (as_seq h0 out);
   lemma_eq_funct_ (as_seq h1 out) (as_seq h0 x)
 
-(*
+
 (* Non constant-time implementations of add_carry_u64 and sub_borrow_u64
    with the same specification as functions in Lib.IntTypes.Intrinsics *)
 
@@ -192,7 +195,7 @@ let le_u64 a b =
   let open Lib.RawIntTypes in
   FStar.UInt64.(u64_to_UInt64 a <=^ u64_to_UInt64 b)
 
-val add_carry_u64_nCT: cin:uint64 -> x:uint64 -> y:uint64 -> r:lbuffer uint64 (size 1) ->
+val add_carry_u64: cin:uint64 -> x:uint64 -> y:uint64 -> r:lbuffer uint64 (size 1) ->
   Stack uint64
     (requires fun h -> live h r /\ v cin <= 1)
     (ensures  fun h0 c h1 ->
@@ -200,16 +203,14 @@ val add_carry_u64_nCT: cin:uint64 -> x:uint64 -> y:uint64 -> r:lbuffer uint64 (s
       (let r = Seq.index (as_seq h1 r) 0 in
        v r + v c * pow2 64 == v x + v y + v cin))
 
-let add_carry_u64_nCT cin x y result1 =
+let add_carry_u64 cin x y result1 =
   let res1 = x +. cin in
-  let mask1 = res1 `lt_mask` cin in
-  lt_mask_lemma res1 cin;
-  let c = copy_conditional_u64 (u64 0) (u64 1) mask1 in
+  let c = (res1 `lt_mask` cin) &. (u64 1) in
+    logand_lemma (lt_mask res1 cin) (u64 1);
   let res = res1 +. y in
-  let mask2 = res `lt_mask` res1 in
-  lt_mask_lemma res res1;
+  let c1 = (res `lt_mask` res1) &. (u64 1) in
+      logand_lemma (lt_mask res res1) (u64 1);
   result1.(0ul) <- res;
-  let c1 = copy_conditional_u64 (u64 0) (u64 1) mask2 in
   c +. c1
 
 val sub_borrow_u64_nCT: cin:uint64 -> x:uint64 -> y:uint64 -> r:lbuffer uint64 (size 1) ->
@@ -230,7 +231,7 @@ let sub_borrow_u64_nCT cin x y result1 =
   in
   result1.(0ul) <- res;
   c
-*)
+
 
 val add4: x: felem -> y: felem -> result: felem -> 
   Stack uint64
